% Generated on 2025-05-29 16:58:28 by gEcon ver. 1.2.3 (2025-04-13)
% http://gecon.r-forge.r-project.org/

% Model name: nRa_chapter4

\section{CONSUMER 1}

\subsection{Optimisation problem}

\begin{align}
&\max_{K^{\mathrm{1}^{\mathrm{s}}}_{t}, C^{\mathrm{1}}_{t}, L^{\mathrm{1}^{\mathrm{s}}}_{t}, I^{\mathrm{1}}_{t}
} U^{\mathrm{1}}_{t} = {\beta} {\mathrm{E}_{t}\left[U^{\mathrm{1}}_{t+1}\right]} + {\gamma} {\log{C^{\mathrm{1}}_{t}}} + {\log\left(1 - L^{\mathrm{1}^{\mathrm{s}}}_{t}\right)} \left(1 - \gamma\right)\\
&\mathrm{s.t.:}\nonumber\\
& C^{\mathrm{1}}_{t} + I^{\mathrm{1}}_{t} = {K^{\mathrm{1}^{\mathrm{s}}}_{t-1}} {r_{t}} + {L^{\mathrm{1}^{\mathrm{s}}}_{t}} {W_{t}} \quad \left(\lambda^{\mathrm{CONSUMER}^{\mathrm{1}^{\mathrm{1}}}}_{t}\right)\\
& K^{\mathrm{1}^{\mathrm{s}}}_{t} = I^{\mathrm{1}}_{t} + {K^{\mathrm{1}^{\mathrm{s}}}_{t-1}} \left(1 - \delta\right) \quad \left(\lambda^{\mathrm{CONSUMER}^{\mathrm{1}^{\mathrm{2}}}}_{t}\right)
\end{align}


\subsection{First order conditions}

\begin{equation}
-\lambda^{\mathrm{CONSUMER}^{\mathrm{1}^{\mathrm{2}}}}_{t} + {\beta} \left(\left(1 - \delta\right) {\mathrm{E}_{t}\left[\lambda^{\mathrm{CONSUMER}^{\mathrm{1}^{\mathrm{2}}}}_{t+1}\right]} + \mathrm{E}_{t}\left[{\lambda^{\mathrm{CONSUMER}^{\mathrm{1}^{\mathrm{1}}}}_{t+1}} {r_{t+1}}\right]\right) = 0
 \quad \left(K^{\mathrm{1}^{\mathrm{s}}}_{t}\right)
\end{equation}
\begin{equation}
-\lambda^{\mathrm{CONSUMER}^{\mathrm{1}^{\mathrm{1}}}}_{t} + {\gamma} {C^{\mathrm{1}}_{t}}^{-1} = 0
 \quad \left(C^{\mathrm{1}}_{t}\right)
\end{equation}
\begin{equation}
{\lambda^{\mathrm{CONSUMER}^{\mathrm{1}^{\mathrm{1}}}}_{t}} {W_{t}} - \left(1 - \gamma\right) \left(1 - L^{\mathrm{1}^{\mathrm{s}}}_{t}\right)^{-1} = 0
 \quad \left(L^{\mathrm{1}^{\mathrm{s}}}_{t}\right)
\end{equation}
\begin{equation}
-\lambda^{\mathrm{CONSUMER}^{\mathrm{1}^{\mathrm{1}}}}_{t} + \lambda^{\mathrm{CONSUMER}^{\mathrm{1}^{\mathrm{2}}}}_{t} = 0
 \quad \left(I^{\mathrm{1}}_{t}\right)
\end{equation}




\section{CONSUMER 2}

\subsection{Optimisation problem}

\begin{align}
&\max_{C^{\mathrm{2}}_{t}, L^{\mathrm{2}^{\mathrm{s}}}_{t}
} U^{\mathrm{2}}_{t} = {\beta} {\mathrm{E}_{t}\left[U^{\mathrm{2}}_{t+1}\right]} + {\gamma} {\log{C^{\mathrm{2}}_{t}}} + {\log\left(1 - L^{\mathrm{2}^{\mathrm{s}}}_{t}\right)} \left(1 - \gamma\right)\\
&\mathrm{s.t.:}\nonumber\\
& C^{\mathrm{2}}_{t} = {L^{\mathrm{2}^{\mathrm{s}}}_{t}} {W_{t}} \quad \left(\lambda^{\mathrm{CONSUMER}^{\mathrm{2}^{\mathrm{1}}}}_{t}\right)
\end{align}


\subsection{First order conditions}

\begin{equation}
-\lambda^{\mathrm{CONSUMER}^{\mathrm{2}^{\mathrm{1}}}}_{t} + {\gamma} {C^{\mathrm{2}}_{t}}^{-1} = 0
 \quad \left(C^{\mathrm{2}}_{t}\right)
\end{equation}
\begin{equation}
{\lambda^{\mathrm{CONSUMER}^{\mathrm{2}^{\mathrm{1}}}}_{t}} {W_{t}} - \left(1 - \gamma\right) \left(1 - L^{\mathrm{2}^{\mathrm{s}}}_{t}\right)^{-1} = 0
 \quad \left(L^{\mathrm{2}^{\mathrm{s}}}_{t}\right)
\end{equation}


\subsection{First order conditions after reduction}

\begin{equation}
-\left(1 - \gamma\right) \left(1 - L^{\mathrm{2}^{\mathrm{s}}}_{t}\right)^{-1} + {\gamma} {C^{\mathrm{2}}_{t}}^{-1} {W_{t}} = 0
 \quad \left(L^{\mathrm{2}^{\mathrm{s}}}_{t}\right)
\end{equation}




\section{AGGREGATION}

\subsection{Identities}

\begin{equation}
C_{t} = {\omega} {C^{\mathrm{1}}_{t}} + {C^{\mathrm{2}}_{t}} \left(1 - \omega\right)
\end{equation}
\begin{equation}
L^{\mathrm{s}}_{t} = {\omega} {L^{\mathrm{1}^{\mathrm{s}}}_{t}} + {L^{\mathrm{2}^{\mathrm{s}}}_{t}} \left(1 - \omega\right)
\end{equation}
\begin{equation}
K^{\mathrm{s}}_{t} = {\omega} {K^{\mathrm{1}^{\mathrm{s}}}_{t}}
\end{equation}
\begin{equation}
I_{t} = {\omega} {I^{\mathrm{1}}_{t}}
\end{equation}




\section{FIRM}

\subsection{Optimisation problem}

\begin{align}
&\max_{K^{\mathrm{d}}_{t}, L^{\mathrm{d}}_{t}, Y_{t}, \pi_{t}
} \Pi_{t} = \pi_{t}\\
&\mathrm{s.t.:}\nonumber\\
& Y_{t} = {A_{t}} {{K^{\mathrm{d}}_{t}}^{\alpha}} {{L^{\mathrm{d}}_{t}}^{1 - \alpha}} \quad \left(\lambda^{\mathrm{FIRM}^{\mathrm{1}}}_{t}\right)\\
& \pi_{t} = Y_{t} - {L^{\mathrm{d}}_{t}} {W_{t}} - {r_{t}} {K^{\mathrm{d}}_{t}} \quad \left(\lambda^{\mathrm{FIRM}^{\mathrm{2}}}_{t}\right)
\end{align}


\subsection{First order conditions}

\begin{equation}
-{\lambda^{\mathrm{FIRM}^{\mathrm{2}}}_{t}} {r_{t}} + {\alpha} {\lambda^{\mathrm{FIRM}^{\mathrm{1}}}_{t}} {A_{t}} {{K^{\mathrm{d}}_{t}}^{-1 + \alpha}} {{L^{\mathrm{d}}_{t}}^{1 - \alpha}} = 0
 \quad \left(K^{\mathrm{d}}_{t}\right)
\end{equation}
\begin{equation}
-{\lambda^{\mathrm{FIRM}^{\mathrm{2}}}_{t}} {W_{t}} + {\lambda^{\mathrm{FIRM}^{\mathrm{1}}}_{t}} {A_{t}} \left(1 - \alpha\right) {{K^{\mathrm{d}}_{t}}^{\alpha}} {{L^{\mathrm{d}}_{t}}^{-\alpha}} = 0
 \quad \left(L^{\mathrm{d}}_{t}\right)
\end{equation}
\begin{equation}
-\lambda^{\mathrm{FIRM}^{\mathrm{1}}}_{t} + \lambda^{\mathrm{FIRM}^{\mathrm{2}}}_{t} = 0
 \quad \left(Y_{t}\right)
\end{equation}
\begin{equation}
1 - \lambda^{\mathrm{FIRM}^{\mathrm{2}}}_{t} = 0
 \quad \left(\pi_{t}\right)
\end{equation}


\subsection{First order conditions after reduction}

\begin{equation}
-r_{t} + {\alpha} {A_{t}} {{K^{\mathrm{d}}_{t}}^{-1 + \alpha}} {{L^{\mathrm{d}}_{t}}^{1 - \alpha}} = 0
 \quad \left(K^{\mathrm{d}}_{t}\right)
\end{equation}
\begin{equation}
-W_{t} + {A_{t}} \left(1 - \alpha\right) {{K^{\mathrm{d}}_{t}}^{\alpha}} {{L^{\mathrm{d}}_{t}}^{-\alpha}} = 0
 \quad \left(L^{\mathrm{d}}_{t}\right)
\end{equation}




\section{EQUILIBRIUM}

\subsection{Identities}

\begin{equation}
K^{\mathrm{d}}_{t} = K^{\mathrm{s}}_{t-1}
\end{equation}
\begin{equation}
L^{\mathrm{d}}_{t} = L^{\mathrm{s}}_{t}
\end{equation}




\section{EXOG}

\subsection{Identities}

\begin{equation}
A_{t} = e^{\epsilon^{\mathrm{A}}_{t} + {\rho} {\log{A_{t-1}}}}
\end{equation}




\section{Equilibrium relationships (after reduction)}

\begin{equation}
-\pi_{t} + \Pi_{t} = 0
\end{equation}
\begin{equation}
-r_{t} + {\alpha} {A_{t}} {{K^{\mathrm{s}}_{t-1}}^{-1 + \alpha}} {{L^{\mathrm{s}}_{t}}^{1 - \alpha}} = 0
\end{equation}
\begin{equation}
-A_{t} + e^{\epsilon^{\mathrm{A}}_{t} + {\rho} {\log{A_{t-1}}}} = 0
\end{equation}
\begin{equation}
-C^{\mathrm{2}}_{t} + {L^{\mathrm{2}^{\mathrm{s}}}_{t}} {W_{t}} = 0
\end{equation}
\begin{equation}
-I_{t} + {\omega} {I^{\mathrm{1}}_{t}} = 0
\end{equation}
\begin{equation}
-K^{\mathrm{s}}_{t} + {\omega} {K^{\mathrm{1}^{\mathrm{s}}}_{t}} = 0
\end{equation}
\begin{equation}
-W_{t} + {A_{t}} \left(1 - \alpha\right) {{K^{\mathrm{s}}_{t-1}}^{\alpha}} {{L^{\mathrm{s}}_{t}}^{-\alpha}} = 0
\end{equation}
\begin{equation}
-Y_{t} + {A_{t}} {{K^{\mathrm{s}}_{t-1}}^{\alpha}} {{L^{\mathrm{s}}_{t}}^{1 - \alpha}} = 0
\end{equation}
\begin{equation}
{\beta} \left({\gamma} {\mathrm{E}_{t}\left[{r_{t+1}} {C^{\mathrm{1}}_{t+1}}^{-1}\right]} + {\gamma} \left(1 - \delta\right) {\mathrm{E}_{t}\left[{C^{\mathrm{1}}_{t+1}}^{-1}\right]}\right) - {\gamma} {C^{\mathrm{1}}_{t}}^{-1} = 0
\end{equation}
\begin{equation}
-\left(1 - \gamma\right) \left(1 - L^{\mathrm{1}^{\mathrm{s}}}_{t}\right)^{-1} + {\gamma} {C^{\mathrm{1}}_{t}}^{-1} {W_{t}} = 0
\end{equation}
\begin{equation}
-\left(1 - \gamma\right) \left(1 - L^{\mathrm{2}^{\mathrm{s}}}_{t}\right)^{-1} + {\gamma} {C^{\mathrm{2}}_{t}}^{-1} {W_{t}} = 0
\end{equation}
\begin{equation}
-C_{t} + {\omega} {C^{\mathrm{1}}_{t}} + {C^{\mathrm{2}}_{t}} \left(1 - \omega\right) = 0
\end{equation}
\begin{equation}
I^{\mathrm{1}}_{t} - K^{\mathrm{1}^{\mathrm{s}}}_{t} + {K^{\mathrm{1}^{\mathrm{s}}}_{t-1}} \left(1 - \delta\right) = 0
\end{equation}
\begin{equation}
-L^{\mathrm{s}}_{t} + {\omega} {L^{\mathrm{1}^{\mathrm{s}}}_{t}} + {L^{\mathrm{2}^{\mathrm{s}}}_{t}} \left(1 - \omega\right) = 0
\end{equation}
\begin{equation}
-\pi_{t} + Y_{t} - {K^{\mathrm{s}}_{t-1}} {r_{t}} - {L^{\mathrm{s}}_{t}} {W_{t}} = 0
\end{equation}
\begin{equation}
-C^{\mathrm{1}}_{t} - I^{\mathrm{1}}_{t} + {K^{\mathrm{1}^{\mathrm{s}}}_{t-1}} {r_{t}} + {L^{\mathrm{1}^{\mathrm{s}}}_{t}} {W_{t}} = 0
\end{equation}
\begin{equation}
U^{\mathrm{1}}_{t} - {\beta} {\mathrm{E}_{t}\left[U^{\mathrm{1}}_{t+1}\right]} - {\gamma} {\log{C^{\mathrm{1}}_{t}}} - {\log\left(1 - L^{\mathrm{1}^{\mathrm{s}}}_{t}\right)} \left(1 - \gamma\right) = 0
\end{equation}
\begin{equation}
U^{\mathrm{2}}_{t} - {\beta} {\mathrm{E}_{t}\left[U^{\mathrm{2}}_{t+1}\right]} - {\gamma} {\log{C^{\mathrm{2}}_{t}}} - {\log\left(1 - L^{\mathrm{2}^{\mathrm{s}}}_{t}\right)} \left(1 - \gamma\right) = 0
\end{equation}



\section{Steady state relationships (after reduction)}

\begin{equation}
-\pi_\mathrm{ss} + \Pi_\mathrm{ss} = 0
\end{equation}
\begin{equation}
-r_\mathrm{ss} + {\alpha} {A_\mathrm{ss}} {{K^{\mathrm{s}}_\mathrm{ss}}^{-1 + \alpha}} {{L^{\mathrm{s}}_\mathrm{ss}}^{1 - \alpha}} = 0
\end{equation}
\begin{equation}
-A_\mathrm{ss} + e^{{\rho} {\log{A_\mathrm{ss}}}} = 0
\end{equation}
\begin{equation}
-C^{\mathrm{2}}_\mathrm{ss} + {L^{\mathrm{2}^{\mathrm{s}}}_\mathrm{ss}} {W_\mathrm{ss}} = 0
\end{equation}
\begin{equation}
-I_\mathrm{ss} + {\omega} {I^{\mathrm{1}}_\mathrm{ss}} = 0
\end{equation}
\begin{equation}
-K^{\mathrm{s}}_\mathrm{ss} + {\omega} {K^{\mathrm{1}^{\mathrm{s}}}_\mathrm{ss}} = 0
\end{equation}
\begin{equation}
-W_\mathrm{ss} + {A_\mathrm{ss}} \left(1 - \alpha\right) {{K^{\mathrm{s}}_\mathrm{ss}}^{\alpha}} {{L^{\mathrm{s}}_\mathrm{ss}}^{-\alpha}} = 0
\end{equation}
\begin{equation}
-Y_\mathrm{ss} + {A_\mathrm{ss}} {{K^{\mathrm{s}}_\mathrm{ss}}^{\alpha}} {{L^{\mathrm{s}}_\mathrm{ss}}^{1 - \alpha}} = 0
\end{equation}
\begin{equation}
{\beta} \left({\gamma} {r_\mathrm{ss}} {C^{\mathrm{1}}_\mathrm{ss}}^{-1} + {\gamma} {C^{\mathrm{1}}_\mathrm{ss}}^{-1} \left(1 - \delta\right)\right) - {\gamma} {C^{\mathrm{1}}_\mathrm{ss}}^{-1} = 0
\end{equation}
\begin{equation}
-\left(1 - \gamma\right) \left(1 - L^{\mathrm{1}^{\mathrm{s}}}_\mathrm{ss}\right)^{-1} + {\gamma} {C^{\mathrm{1}}_\mathrm{ss}}^{-1} {W_\mathrm{ss}} = 0
\end{equation}
\begin{equation}
-\left(1 - \gamma\right) \left(1 - L^{\mathrm{2}^{\mathrm{s}}}_\mathrm{ss}\right)^{-1} + {\gamma} {C^{\mathrm{2}}_\mathrm{ss}}^{-1} {W_\mathrm{ss}} = 0
\end{equation}
\begin{equation}
-C_\mathrm{ss} + {\omega} {C^{\mathrm{1}}_\mathrm{ss}} + {C^{\mathrm{2}}_\mathrm{ss}} \left(1 - \omega\right) = 0
\end{equation}
\begin{equation}
I^{\mathrm{1}}_\mathrm{ss} - K^{\mathrm{1}^{\mathrm{s}}}_\mathrm{ss} + {K^{\mathrm{1}^{\mathrm{s}}}_\mathrm{ss}} \left(1 - \delta\right) = 0
\end{equation}
\begin{equation}
-L^{\mathrm{s}}_\mathrm{ss} + {\omega} {L^{\mathrm{1}^{\mathrm{s}}}_\mathrm{ss}} + {L^{\mathrm{2}^{\mathrm{s}}}_\mathrm{ss}} \left(1 - \omega\right) = 0
\end{equation}
\begin{equation}
-\pi_\mathrm{ss} + Y_\mathrm{ss} - {r_\mathrm{ss}} {K^{\mathrm{s}}_\mathrm{ss}} - {L^{\mathrm{s}}_\mathrm{ss}} {W_\mathrm{ss}} = 0
\end{equation}
\begin{equation}
-C^{\mathrm{1}}_\mathrm{ss} - I^{\mathrm{1}}_\mathrm{ss} + {r_\mathrm{ss}} {K^{\mathrm{1}^{\mathrm{s}}}_\mathrm{ss}} + {L^{\mathrm{1}^{\mathrm{s}}}_\mathrm{ss}} {W_\mathrm{ss}} = 0
\end{equation}
\begin{equation}
U^{\mathrm{1}}_\mathrm{ss} - {\beta} {U^{\mathrm{1}}_\mathrm{ss}} - {\gamma} {\log{C^{\mathrm{1}}_\mathrm{ss}}} - {\log\left(1 - L^{\mathrm{1}^{\mathrm{s}}}_\mathrm{ss}\right)} \left(1 - \gamma\right) = 0
\end{equation}
\begin{equation}
U^{\mathrm{2}}_\mathrm{ss} - {\beta} {U^{\mathrm{2}}_\mathrm{ss}} - {\gamma} {\log{C^{\mathrm{2}}_\mathrm{ss}}} - {\log\left(1 - L^{\mathrm{2}^{\mathrm{s}}}_\mathrm{ss}\right)} \left(1 - \gamma\right) = 0
\end{equation}






\section{Parameter settings}

\begin{equation}
\alpha = 0.35
\end{equation}
\begin{equation}
\beta = 0.97
\end{equation}
\begin{equation}
\delta = 0.06
\end{equation}
\begin{equation}
\gamma = 0.4
\end{equation}
\begin{equation}
\omega = 0.5
\end{equation}
\begin{equation}
\rho = 0.95
\end{equation}


