% Generated on 2025-05-29 16:04:00 by gEcon ver. 1.2.3 (2025-04-13)
% http://gecon.r-forge.r-project.org/

% Model name: Taxes_chapter7_multiple_shocks

\section{CONSUMER}

\subsection{Optimisation problem}

\begin{align}
&\max_{K^{\mathrm{s}}_{t}, C_{t}, L^{\mathrm{s}}_{t}, I_{t}
} U_{t} = {\beta} {\mathrm{E}_{t}\left[U_{t+1}\right]} + {\gamma} {\log{C_{t}}} + {\log\left(1 - L^{\mathrm{s}}_{t}\right)} \left(1 - \gamma\right)\\
&\mathrm{s.t.:}\nonumber\\
& I_{t} + {C_{t}} \left(1 + \tau^{\mathrm{c}}\right) = \pi_{t} + {G\!T}_{t} + {K^{\mathrm{s}}_{t-1}} {r_{t}} \left(1 - \tau^{\mathrm{k}}\right) + {L^{\mathrm{s}}_{t}} {W_{t}} \left(1 - \tau^{\mathrm{l}}\right) \quad \left(\lambda^{\mathrm{c}}_{t}\right)\\
& K^{\mathrm{s}}_{t} = I_{t} + {K^{\mathrm{s}}_{t-1}} \left(1 - \delta\right) \quad \left(\lambda^{\mathrm{CONSUMER}^{\mathrm{2}}}_{t}\right)
\end{align}


\subsection{First order conditions}

\begin{equation}
-\lambda^{\mathrm{CONSUMER}^{\mathrm{2}}}_{t} + {\beta} \left(\left(1 - \delta\right) {\mathrm{E}_{t}\left[\lambda^{\mathrm{CONSUMER}^{\mathrm{2}}}_{t+1}\right]} + \left(1 - \tau^{\mathrm{k}}\right) {\mathrm{E}_{t}\left[{\lambda^{\mathrm{c}}_{t+1}} {r_{t+1}}\right]}\right) = 0
 \quad \left(K^{\mathrm{s}}_{t}\right)
\end{equation}
\begin{equation}
{\gamma} {C_{t}}^{-1} + {\lambda^{\mathrm{c}}_{t}} \left(-1 - \tau^{\mathrm{c}}\right) = 0
 \quad \left(C_{t}\right)
\end{equation}
\begin{equation}
-\left(1 - \gamma\right) \left(1 - L^{\mathrm{s}}_{t}\right)^{-1} + {\lambda^{\mathrm{c}}_{t}} {W_{t}} \left(1 - \tau^{\mathrm{l}}\right) = 0
 \quad \left(L^{\mathrm{s}}_{t}\right)
\end{equation}
\begin{equation}
-\lambda^{\mathrm{c}}_{t} + \lambda^{\mathrm{CONSUMER}^{\mathrm{2}}}_{t} = 0
 \quad \left(I_{t}\right)
\end{equation}




\section{FIRM}

\subsection{Optimisation problem}

\begin{align}
&\max_{K^{\mathrm{d}}_{t}, L^{\mathrm{d}}_{t}, Y_{t}, \pi_{t}
} \Pi_{t} = \pi_{t}\\
&\mathrm{s.t.:}\nonumber\\
& Y_{t} = {A_{t}} {{K^{\mathrm{d}}_{t}}^{\alpha}} {{L^{\mathrm{d}}_{t}}^{1 - \alpha}} \quad \left(\lambda^{\mathrm{FIRM}^{\mathrm{1}}}_{t}\right)\\
& \pi_{t} = Y_{t} - {L^{\mathrm{d}}_{t}} {W_{t}} - {r_{t}} {K^{\mathrm{d}}_{t}} \quad \left(\lambda^{\mathrm{FIRM}^{\mathrm{2}}}_{t}\right)
\end{align}


\subsection{First order conditions}

\begin{equation}
-{\lambda^{\mathrm{FIRM}^{\mathrm{2}}}_{t}} {r_{t}} + {\alpha} {\lambda^{\mathrm{FIRM}^{\mathrm{1}}}_{t}} {A_{t}} {{K^{\mathrm{d}}_{t}}^{-1 + \alpha}} {{L^{\mathrm{d}}_{t}}^{1 - \alpha}} = 0
 \quad \left(K^{\mathrm{d}}_{t}\right)
\end{equation}
\begin{equation}
-{\lambda^{\mathrm{FIRM}^{\mathrm{2}}}_{t}} {W_{t}} + {\lambda^{\mathrm{FIRM}^{\mathrm{1}}}_{t}} {A_{t}} \left(1 - \alpha\right) {{K^{\mathrm{d}}_{t}}^{\alpha}} {{L^{\mathrm{d}}_{t}}^{-\alpha}} = 0
 \quad \left(L^{\mathrm{d}}_{t}\right)
\end{equation}
\begin{equation}
-\lambda^{\mathrm{FIRM}^{\mathrm{1}}}_{t} + \lambda^{\mathrm{FIRM}^{\mathrm{2}}}_{t} = 0
 \quad \left(Y_{t}\right)
\end{equation}
\begin{equation}
1 - \lambda^{\mathrm{FIRM}^{\mathrm{2}}}_{t} = 0
 \quad \left(\pi_{t}\right)
\end{equation}


\subsection{First order conditions after reduction}

\begin{equation}
-r_{t} + {\alpha} {A_{t}} {{K^{\mathrm{d}}_{t}}^{-1 + \alpha}} {{L^{\mathrm{d}}_{t}}^{1 - \alpha}} = 0
 \quad \left(K^{\mathrm{d}}_{t}\right)
\end{equation}
\begin{equation}
-W_{t} + {A_{t}} \left(1 - \alpha\right) {{K^{\mathrm{d}}_{t}}^{\alpha}} {{L^{\mathrm{d}}_{t}}^{-\alpha}} = 0
 \quad \left(L^{\mathrm{d}}_{t}\right)
\end{equation}




\section{GOVERNMENT}

\subsection{Identities}

\begin{equation}
{G\!T}_{t} = G^{\mathrm{inc}}_{t}
\end{equation}
\begin{equation}
G^{\mathrm{inc}}_{t} = T^{\mathrm{c}}_{t} + T^{\mathrm{l}}_{t} + T^{\mathrm{k}}_{t}
\end{equation}
\begin{equation}
T^{\mathrm{c}}_{t} = {\tau^{\mathrm{c}}} {C_{t}}
\end{equation}
\begin{equation}
T^{\mathrm{l}}_{t} = {\tau^{\mathrm{l}}} {L^{\mathrm{s}}_{t}} {W_{t}}
\end{equation}
\begin{equation}
T^{\mathrm{k}}_{t} = {\tau^{\mathrm{k}}} {K^{\mathrm{s}}_{t-1}} \left(-\delta + r_{t}\right)
\end{equation}




\section{EQUILIBRIUM}

\subsection{Identities}

\begin{equation}
K^{\mathrm{d}}_{t} = K^{\mathrm{s}}_{t-1}
\end{equation}
\begin{equation}
L^{\mathrm{d}}_{t} = L^{\mathrm{s}}_{t}
\end{equation}




\section{EXOG}

\subsection{Identities}

\begin{equation}
A_{t} = e^{\epsilon^{\mathrm{A}}_{t} + {\rho} {\log{A_{t-1}}}}
\end{equation}




\section{Equilibrium relationships (after reduction)}

\begin{equation}
-\lambda^{\mathrm{c}}_{t} + {\beta} \left(\left(1 - \delta\right) {\mathrm{E}_{t}\left[\lambda^{\mathrm{c}}_{t+1}\right]} + \left(1 - \tau^{\mathrm{k}}\right) {\mathrm{E}_{t}\left[{\lambda^{\mathrm{c}}_{t+1}} {r_{t+1}}\right]}\right) = 0
\end{equation}
\begin{equation}
-\pi_{t} + \Pi_{t} = 0
\end{equation}
\begin{equation}
-r_{t} + {\alpha} {A_{t}} {{K^{\mathrm{s}}_{t-1}}^{-1 + \alpha}} {{L^{\mathrm{s}}_{t}}^{1 - \alpha}} = 0
\end{equation}
\begin{equation}
-A_{t} + e^{\epsilon^{\mathrm{A}}_{t} + {\rho} {\log{A_{t-1}}}} = 0
\end{equation}
\begin{equation}
G^{\mathrm{inc}}_{t} - {G\!T}_{t} = 0
\end{equation}
\begin{equation}
-T^{\mathrm{c}}_{t} + {\tau^{\mathrm{c}}} {C_{t}} = 0
\end{equation}
\begin{equation}
-T^{\mathrm{l}}_{t} + {\tau^{\mathrm{l}}} {L^{\mathrm{s}}_{t}} {W_{t}} = 0
\end{equation}
\begin{equation}
-T^{\mathrm{k}}_{t} + {\tau^{\mathrm{k}}} {K^{\mathrm{s}}_{t-1}} \left(-\delta + r_{t}\right) = 0
\end{equation}
\begin{equation}
-W_{t} + {A_{t}} \left(1 - \alpha\right) {{K^{\mathrm{s}}_{t-1}}^{\alpha}} {{L^{\mathrm{s}}_{t}}^{-\alpha}} = 0
\end{equation}
\begin{equation}
-Y_{t} + {A_{t}} {{K^{\mathrm{s}}_{t-1}}^{\alpha}} {{L^{\mathrm{s}}_{t}}^{1 - \alpha}} = 0
\end{equation}
\begin{equation}
{\gamma} {C_{t}}^{-1} + {\lambda^{\mathrm{c}}_{t}} \left(-1 - \tau^{\mathrm{c}}\right) = 0
\end{equation}
\begin{equation}
-\left(1 - \gamma\right) \left(1 - L^{\mathrm{s}}_{t}\right)^{-1} + {\lambda^{\mathrm{c}}_{t}} {W_{t}} \left(1 - \tau^{\mathrm{l}}\right) = 0
\end{equation}
\begin{equation}
I_{t} - K^{\mathrm{s}}_{t} + {K^{\mathrm{s}}_{t-1}} \left(1 - \delta\right) = 0
\end{equation}
\begin{equation}
-\pi_{t} + Y_{t} - {K^{\mathrm{s}}_{t-1}} {r_{t}} - {L^{\mathrm{s}}_{t}} {W_{t}} = 0
\end{equation}
\begin{equation}
-G^{\mathrm{inc}}_{t} + T^{\mathrm{c}}_{t} + T^{\mathrm{l}}_{t} + T^{\mathrm{k}}_{t} = 0
\end{equation}
\begin{equation}
U_{t} - {\beta} {\mathrm{E}_{t}\left[U_{t+1}\right]} - {\gamma} {\log{C_{t}}} - {\log\left(1 - L^{\mathrm{s}}_{t}\right)} \left(1 - \gamma\right) = 0
\end{equation}
\begin{equation}
\pi_{t} + {G\!T}_{t} - I_{t} - {C_{t}} \left(1 + \tau^{\mathrm{c}}\right) + {K^{\mathrm{s}}_{t-1}} {r_{t}} \left(1 - \tau^{\mathrm{k}}\right) + {L^{\mathrm{s}}_{t}} {W_{t}} \left(1 - \tau^{\mathrm{l}}\right) = 0
\end{equation}



\section{Steady state relationships (after reduction)}

\begin{equation}
-\lambda^{\mathrm{c}}_\mathrm{ss} + {\beta} \left({\lambda^{\mathrm{c}}_\mathrm{ss}} \left(1 - \delta\right) + {\lambda^{\mathrm{c}}_\mathrm{ss}} {r_\mathrm{ss}} \left(1 - \tau^{\mathrm{k}}\right)\right) = 0
\end{equation}
\begin{equation}
-\pi_\mathrm{ss} + \Pi_\mathrm{ss} = 0
\end{equation}
\begin{equation}
-r_\mathrm{ss} + {\alpha} {A_\mathrm{ss}} {{K^{\mathrm{s}}_\mathrm{ss}}^{-1 + \alpha}} {{L^{\mathrm{s}}_\mathrm{ss}}^{1 - \alpha}} = 0
\end{equation}
\begin{equation}
-A_\mathrm{ss} + e^{{\rho} {\log{A_\mathrm{ss}}}} = 0
\end{equation}
\begin{equation}
G^{\mathrm{inc}}_\mathrm{ss} - {G\!T}_\mathrm{ss} = 0
\end{equation}
\begin{equation}
-T^{\mathrm{c}}_\mathrm{ss} + {\tau^{\mathrm{c}}} {C_\mathrm{ss}} = 0
\end{equation}
\begin{equation}
-T^{\mathrm{l}}_\mathrm{ss} + {\tau^{\mathrm{l}}} {L^{\mathrm{s}}_\mathrm{ss}} {W_\mathrm{ss}} = 0
\end{equation}
\begin{equation}
-T^{\mathrm{k}}_\mathrm{ss} + {\tau^{\mathrm{k}}} {K^{\mathrm{s}}_\mathrm{ss}} \left(-\delta + r_\mathrm{ss}\right) = 0
\end{equation}
\begin{equation}
-W_\mathrm{ss} + {A_\mathrm{ss}} \left(1 - \alpha\right) {{K^{\mathrm{s}}_\mathrm{ss}}^{\alpha}} {{L^{\mathrm{s}}_\mathrm{ss}}^{-\alpha}} = 0
\end{equation}
\begin{equation}
-Y_\mathrm{ss} + {A_\mathrm{ss}} {{K^{\mathrm{s}}_\mathrm{ss}}^{\alpha}} {{L^{\mathrm{s}}_\mathrm{ss}}^{1 - \alpha}} = 0
\end{equation}
\begin{equation}
{\gamma} {C_\mathrm{ss}}^{-1} + {\lambda^{\mathrm{c}}_\mathrm{ss}} \left(-1 - \tau^{\mathrm{c}}\right) = 0
\end{equation}
\begin{equation}
-\left(1 - \gamma\right) \left(1 - L^{\mathrm{s}}_\mathrm{ss}\right)^{-1} + {\lambda^{\mathrm{c}}_\mathrm{ss}} {W_\mathrm{ss}} \left(1 - \tau^{\mathrm{l}}\right) = 0
\end{equation}
\begin{equation}
I_\mathrm{ss} - K^{\mathrm{s}}_\mathrm{ss} + {K^{\mathrm{s}}_\mathrm{ss}} \left(1 - \delta\right) = 0
\end{equation}
\begin{equation}
-\pi_\mathrm{ss} + Y_\mathrm{ss} - {r_\mathrm{ss}} {K^{\mathrm{s}}_\mathrm{ss}} - {L^{\mathrm{s}}_\mathrm{ss}} {W_\mathrm{ss}} = 0
\end{equation}
\begin{equation}
-G^{\mathrm{inc}}_\mathrm{ss} + T^{\mathrm{c}}_\mathrm{ss} + T^{\mathrm{l}}_\mathrm{ss} + T^{\mathrm{k}}_\mathrm{ss} = 0
\end{equation}
\begin{equation}
U_\mathrm{ss} - {\beta} {U_\mathrm{ss}} - {\gamma} {\log{C_\mathrm{ss}}} - {\log\left(1 - L^{\mathrm{s}}_\mathrm{ss}\right)} \left(1 - \gamma\right) = 0
\end{equation}
\begin{equation}
\pi_\mathrm{ss} + {G\!T}_\mathrm{ss} - I_\mathrm{ss} - {C_\mathrm{ss}} \left(1 + \tau^{\mathrm{c}}\right) + {r_\mathrm{ss}} {K^{\mathrm{s}}_\mathrm{ss}} \left(1 - \tau^{\mathrm{k}}\right) + {L^{\mathrm{s}}_\mathrm{ss}} {W_\mathrm{ss}} \left(1 - \tau^{\mathrm{l}}\right) = 0
\end{equation}






\section{Parameter settings}

\begin{equation}
\alpha = 0.35
\end{equation}
\begin{equation}
\beta = 0.97
\end{equation}
\begin{equation}
\delta = 0.06
\end{equation}
\begin{equation}
\gamma = 0.4
\end{equation}
\begin{equation}
\rho = 0.95
\end{equation}
\begin{equation}
\tau^{\mathrm{c}} = 0.116
\end{equation}
\begin{equation}
\tau^{\mathrm{k}} = 0.225
\end{equation}
\begin{equation}
\tau^{\mathrm{l}} = 0.348
\end{equation}


